\documentclass{article}
\usepackage{ifthen}
\usepackage{epsfig}
\usepackage[utf8]{inputenc}
\usepackage{newunicodechar}
  \newunicodechar{⁻}{${}^{-}$}% Superscript minus
  \newunicodechar{²}{${}^{2}$}% Superscript two
  \newunicodechar{³}{${}^{3}$}% Superscript three

\pagestyle{empty}
\begin{document}
$ \ln(Z) $
\pagebreak

$ \ln(Z)/3 + f_c $
\pagebreak

$ ((Fel-fc)+Finel*invZ)$
\pagebreak

$ (Fel-fc)$
\pagebreak

$ (1.0+invZ)/12 $
\pagebreak

$E_\mathrm{sp}-E_\mathrm{i,A}$
\pagebreak

$E_\mathrm{sp}$
\pagebreak

$E_\mathrm{i,A}$
\pagebreak

$A$
\pagebreak

$b$
\pagebreak

\[ r(\theta) = \frac{(1-e^2)r_0/2}{1-e \sin(\theta-\theta_R/2)}, \]
\pagebreak

$e$
\pagebreak

\[ e = \sqrt{1+4b^2/r_0^2}; \]
\pagebreak

$\theta_R$
\pagebreak

\[ \theta_R = \pi - 2\arctan\left(\frac{2b}{r_0}\right) \]
\pagebreak

$\theta$
\pagebreak

$\pi$
\pagebreak

$r_0$
\pagebreak

\[ p_{CM}^2 = \frac{z^2 - m_1^2 m_2^2}{2 z + m_1^2 + m_2^2} \]
\pagebreak

$z$
\pagebreak

\[ z = E_1 E_2 - \vec{p}_1\cdot\vec{p}_2 \]
\pagebreak

\[ p_{lab}^2 = \frac{s^2 - 2 s (m_1^2 + m_2^2) + {(m_1^2 - m_2^2)}^2}{4 m_2^2} \]
\pagebreak

\[ {\left(2.38\cdot\frac{9\pi}{2}\right)}^{1/6}\sqrt\hbar \]
\pagebreak

$2.38h$
\pagebreak

\[ \exp(B\cdot t) \]
\pagebreak

$t$
\pagebreak

$B$
\pagebreak

$\exp(Bt)$
\pagebreak

\[ (0, \Delta\vec{x}), \]
\pagebreak

$\Delta\vec{x}$
\pagebreak

\[ (\Delta t', \Delta\vec{x}'), \]
\pagebreak

\[ |\Delta\vec{x}'| \leq \sqrt{\sigma/\pi}.\]
\pagebreak

$|\Delta\vec{x}'|\leq|\Delta\vec{x}|$
\pagebreak

$\exp(B\cdot t)$
\pagebreak

$\hbar$
\pagebreak

$\hbar c$
\pagebreak

$\hbar^2 c^2$
\pagebreak

\[ e^2/(4 pi epsilon_0) \]
\pagebreak

$\int_{x_0}^{x_1} f(x) dx$
\pagebreak

\[ m = \sqrt{E^2 - {\vec p}^2}\]
\pagebreak

\[ (A_1,Z_1) + (A_2, Z_2) --> (A_1+A_2,Z_1+Z_2) \]
\pagebreak

\[ (A_1,Z_1) + (A_2, Z_2) --> (A_3,Z_3) + (A1+A2-A3,Z1+Z2-Z3) \]
\pagebreak

\[ p_F(A)=\alpha-\beta\cdot e^{(-A\cdot\gamma)} \]
\pagebreak

$\alpha=259.416$
\pagebreak

$c$
\pagebreak

$\beta=152.824$
\pagebreak

$\gamma=9.5157\cdot10^{-2}$
\pagebreak

\[ L = \frac{[K + (K^2 - 1)^\frac{1}{2}]}{a} \]
\pagebreak

\[ K = 1 + \frac{b}{8a} \]
\pagebreak

\[ M = a*L-1 \]
\pagebreak

\end{document}
